roscore.v
@@ -69,7 +69,7 @@ Definition transport {T:Type} {a b:T} {P:T -> Type} (eq:a=b) (pa: P a) : (P b):=
 @eq_rect T a P pa b eq.
 
 
-Definition getPayLoadR  (topic : RosTopic) (m : sigT topicType) :
+Definition getPayloadR  (topic : RosTopic) (m : sigT topicType) :
 option (topicType topic) :=
 match m with
 | (existT tp pl) => match (eqdec  tp topic) with
@@ -78,8 +78,8 @@ match m with
                   end
 end.
 
-Definition getPayLoad  (topic : RosTopic) (m : Message) :
-option (topicType topic) := getPayLoadR topic (fst m).
+Definition getPayload  (topic : RosTopic) (m : Message) :
+option (topicType topic) := getPayloadR topic (fst m).
 
 Definition defHdr :=  mkHeader 0.
 
@@ -94,7 +94,7 @@ Definition liftToMesg {InTopic OutTopic}
   (f : SimplePureProcess InTopic OutTopic) 
     : Message -> (list Message) :=
 ( fun inpMesg : Message => 
-match (getPayLoad InTopic inpMesg ) with
+match (getPayload InTopic inpMesg ) with
 | Some tmesg => cons ((mkImmMesg _ (f tmesg))) nil
 | None => nil
 end).
@@ -106,8 +106,10 @@ Definition mtopicR (m : sigT topicType) :=
 Definition mtopic (m : Message) := 
 mtopicR (fst m).
 
-Definition mPayLoad (m : Message) : topicType (mtopic m) :=
+Definition mPayload (m : Message) : topicType (mtopic m) :=
 (proj2_sigT _ _ (fst m)).
+
+Definition getPayloadOp t := opBind (getPayload t).
 
 Definition validRecvMesg (rn : TopicInfo) (lm : list Message) :=
 ∀ m, In m (map fst lm) -> In (mtopicR m) (subscribeTopics rn).
@@ -132,11 +134,11 @@ Defined.
 
 Definition filterMegsByTopic (lm : list Message) 
   (topic : RosTopic) : list ( (topicType topic)) :=
-flat_map (fun m => op2List (getPayLoad topic m)) lm.
+flat_map (fun m => op2List (getPayload topic m)) lm.
 
 Lemma moveMapInsideFst : forall tp lm,
-  opBind (getPayLoad tp)  (head lm)
-  = opBind (getPayLoadR tp) (head (map fst lm)).
+  opBind (getPayload tp)  (head lm)
+  = opBind (getPayloadR tp) (head (map fst lm)).
 Proof.
   intros ?. destruct lm; reflexivity.
 Qed.
@@ -148,7 +150,7 @@ Definition PureProcWDelay (inT outT : RosTopic)
 Definition delayedLift2Mesg {InTopic OutTopic} 
   (f : PureProcWDelay InTopic OutTopic) 
    (inpMesg : Message) : (list Message) :=
-  match (getPayLoad InTopic inpMesg ) with
+  match (getPayload InTopic inpMesg ) with
   | Some tmesg => map (λ p, (mkDelayedMesg (π₁ p) (π₂ p))) (f tmesg)
   | None => nil
   end.
